src/Arithmetic/BYInv/Firstn.v
@@ -1,0 +1,54 @@
+Require Import Coq.ZArith.ZArith.
+Require Import Coq.micromega.Lia.
+Require Import Coq.Lists.List.
+
+Require Import Crypto.Arithmetic.UniformWeight.
+Require Import Crypto.Arithmetic.Saturated.
+Require Import Crypto.Arithmetic.Core.
+
+Require Import Crypto.Arithmetic.BYInv.EvalLemmas.
+Require Import Crypto.Arithmetic.BYInv.Definitions.
+
+Require Import Crypto.Util.ZUtil.Definitions.
+Require Import Crypto.Util.ZUtil.TwosComplement.
+
+Require Import Crypto.Util.ListUtil.
+Require Import Crypto.Util.LetIn.
+
+
+Import Positional.
+
+Local Open Scope Z_scope.
+Local Coercion Z.of_nat : nat >-> Z.
+
+Lemma firstn_eval m n f k
+      (Hm : 0 < m)
+      (Hf : length f = n)
+      (Hf2 : forall z : Z, In z f -> 0 <= z < 2 ^ m)
+      (Hk : (k <= n)%nat) :
+  eval (uweight m) k (firstn k f) = eval (uweight m) n f mod 2 ^ (m * k).
+Proof.
+  rewrite <- (firstn_skipn k f) at 2.
+  replace n with (k + length (skipn k f))%nat by (rewrite skipn_length; lia).
+  rewrite (uweight_eval_app' m ltac:(lia) k), uweight_eq_alt, <- Z.pow_mul_r
+    by (rewrite ?firstn_length, ?Nat.min_l; lia).
+  autorewrite with push_Zmod.
+  rewrite Z.mod_0_l, Z.add_0_r,  Z.mod_mod
+    by (try apply Z.pow_nonzero; nia).
+  rewrite Z.mod_small. reflexivity.
+  apply eval_bound. lia. intros.
+  apply Hf2. apply (In_firstn k).  assumption.
+  rewrite firstn_length, Nat.min_l. reflexivity. lia.
+Qed.
+
+Lemma firstn_tc_eval m n f k
+      (Hm : 0 < m)
+      (Hf : length f = n)
+      (Hf2 : forall z : Z, In z f -> 0 <= z < 2 ^ m)
+      (Hk : (0 < k <= n)%nat) :
+  tc_eval m k (firstn k f) = Z.twos_complement (m * k) (tc_eval m n f).
+Proof.
+  unfold tc_eval.
+  rewrite firstn_eval with (n:=n), Z.twos_complement_mod, Z.twos_complement_twos_complement_smaller_width;
+    nia || reflexivity || assumption.
+Qed.
