src/Arithmetic/BYInv/One.v
@@ -1,0 +1,30 @@
+Require Import Coq.ZArith.ZArith.
+Require Import Coq.micromega.Lia.
+Require Import Coq.Lists.List.
+
+Require Import Crypto.Arithmetic.BYInv.Definitions.
+
+Require Import Crypto.Arithmetic.UniformWeight.
+Require Import Crypto.Arithmetic.Saturated.
+Require Import Crypto.Arithmetic.Core.
+
+Import Positional.
+Import Crypto.Util.ZUtil.Notations.
+
+Local Open Scope Z_scope.
+
+Lemma length_one n (Hn : (0 < n)%nat) :
+  length (one n) = n.
+Proof. unfold one; simpl; rewrite length_zeros; lia. Qed.
+
+Hint Rewrite length_one : distr_length.
+
+Lemma eval_one n machine_wordsize
+      (Hn : (0 < n)%nat)
+      (Hmw : 0 <= machine_wordsize) :
+  eval (uweight machine_wordsize) n (one n) = 1.
+Proof.
+  unfold one. destruct n. lia.
+  rewrite eval_cons, uweight_eval_shift, uweight_0, uweight_1 by (try rewrite length_zeros; lia).
+  replace (S n - 1)%nat with n by lia. rewrite eval_zeros; lia.
+Qed.
