src/Arithmetic/BYInv/Select.v
@@ -1,0 +1,25 @@
+Require Import Coq.ZArith.ZArith.
+Require Import Coq.micromega.Lia.
+Require Import Coq.Lists.List.
+
+Require Import Crypto.Arithmetic.BYInv.Definitions.
+
+Require Import Crypto.Arithmetic.UniformWeight.
+Require Import Crypto.Arithmetic.Saturated.
+Require Import Crypto.Arithmetic.Core.
+
+Require Import Crypto.Util.Decidable.
+
+Import Positional.
+Import Crypto.Util.ZUtil.Notations.
+
+Local Open Scope Z_scope.
+Local Coercion Z.of_nat : nat >-> Z.
+
+Lemma tc_eval_select machine_wordsize n cond f g
+      (Hf : length f = n)
+      (Hg : length g = n) :
+  tc_eval machine_wordsize n (select cond f g) = if dec (cond = 0)
+                                                    then (tc_eval machine_wordsize n f)
+                                                    else (tc_eval machine_wordsize n g).
+Proof. unfold tc_eval; rewrite eval_select; auto; destruct (dec (cond = 0)); auto. Qed.
