src/Util/ZUtil/TwosComplementOpp.v
@@ -1,0 +1,60 @@
+Require Import Coq.ZArith.ZArith.
+Require Import Coq.micromega.Lia.
+
+Require Import Crypto.Util.ZUtil.Definitions.
+Require Import Crypto.Util.ZUtil.TwosComplement.
+Require Import Crypto.Util.ZUtil.Odd.
+Require Import Crypto.Util.ZUtil.AddGetCarry.
+
+Local Open Scope Z_scope.
+
+Section Z.
+
+  Lemma twos_complement_opp_bound m a (Hm : 0 <= m) :
+    0 <= Z.twos_complement_opp m a < 2 ^ m.
+  Proof. unfold Z.twos_complement_opp; apply Z.mod_pos_bound.
+         apply Z.pow_pos_nonneg; lia.
+  Qed.
+
+  Lemma twos_complement_opp_correct m a :
+    (Z.twos_complement_opp m a) = - a mod 2 ^ m.
+  Proof. unfold Z.twos_complement_opp, Z.lnot_modulo, Z.lnot.
+         rewrite Zplus_mod_idemp_l, <- Z.sub_1_r; apply f_equal2; lia.
+  Qed.
+
+  Lemma twos_complement_zopp a m (Hm : 0 < m) (corner_case : Z.twos_complement m a <> - 2 ^ (m - 1)) :
+    Z.twos_complement m (- a) = - Z.twos_complement m a.
+  Proof.
+    pose proof Z.twos_complement_bounds m a Hm.
+    apply Z.twos_complement_spec; [lia|split]; [|lia].
+    rewrite (PullPush.Z.opp_mod_mod (Z.twos_complement _ _)), Z.twos_complement_mod' by lia;
+      apply PullPush.Z.opp_mod_mod.
+  Qed.
+
+  Lemma twos_complement_opp_spec m a
+        (Hm : 0 < m) (corner_case : Z.twos_complement m a <> - 2 ^ (m - 1)) :
+    Z.twos_complement m (Z.twos_complement_opp m a) = - (Z.twos_complement m a).
+  Proof.
+    apply Z.twos_complement_spec; [lia|split]; [|pose proof Z.twos_complement_bounds m a Hm; lia].
+    now rewrite <- twos_complement_zopp, twos_complement_opp_correct, Z.twos_complement_mod', Z.mod_mod by (try apply Z.pow_nonzero; lia).
+  Qed.
+
+  Lemma twos_complement_opp_odd m a (Hm : 0 < m) (aodd : Z.odd a = true) :
+    Z.odd (Z.twos_complement_opp m a) = true.
+  Proof.
+    unfold Z.twos_complement_opp, Z.lnot_modulo, Z.lnot.
+    rewrite Zplus_mod_idemp_l.
+    replace (Z.pred (- a) + 1) with (-a) by lia.
+    now rewrite Z.odd_mod2m, Z.odd_opp by assumption.
+  Qed.
+
+  Lemma twos_complement_opp'_spec m a :
+    Z.twos_complement_opp' m a = Z.twos_complement_opp m a.
+  Proof.
+    unfold Z.twos_complement_opp', Z.twos_complement_opp.
+    destruct (Z_lt_dec m 0).
+    - rewrite !Z.pow_neg_r, !Zmod_0_r by assumption; reflexivity.
+    - rewrite Z.add_get_carry_full_mod; auto with zarith.
+  Qed.
+
+End Z.
